Initial implementation of concurrency interface v2

src/Values.v
@@ -1340,6 +1340,26 @@ Definition vector_init {T} (n : Z) (t : T) : vec T n :=
 
 #[export] Instance dummy_vec {T:Type} `{Inhabited T} n : Inhabited (vec T n) := {| inhabitant := vector_init n inhabitant |}.
 
+Fixpoint list_init {T} n (f : Z -> T) : list T :=
+match n with
+| O => []
+| S m => f (Z.of_nat m) :: list_init m f
+end.
+
+Lemma list_init_length T n (f : Z -> T) :
+  length (list_init n f) = n.
+Proof.
+  induction n.
+  - reflexivity.
+  - simpl. auto.
+Qed.
+
+Definition vec_init_fn {T} n (f : Z -> T) : vec T n :=
+  match sumbool_of_bool (n >=? 0) with
+  | left GE => @existT _ _ (list_init (Z.to_nat n) f) (list_init_length _ _ _)
+  | right NGE => dodgy_vec n NGE
+  end.
+
 Definition vec_concat {T m n} `{Inhabited T} (v : vec T m) (w : vec T n) : vec T (m + n).
 refine (
   if sumbool_of_bool ((m >=? 0) && (n >=? 0)) then
