src-stdpp/ConcurrencyInterfaceBuiltinsV2.v
@@ -1,0 +1,416 @@
+Require Import Real Base ConcurrencyInterfaceTypesV2 ConcurrencyInterfaceV2.
+From stdpp Require Import bitvector.definitions.
+
+Import ListNotations.
+Open Scope string.
+Open Scope bool.
+Open Scope Z.
+
+Module Defs (A : Arch) (I : InterfaceT A).
+
+Definition monad E := I.iMon (fun _ => E).
+Definition returnm {A E} : A -> monad E A := I.Ret.
+
+Definition monadR R E := I.iMon (fun _ => (R + E)%type).
+Definition returnR {A E} R : A -> monadR R E A := I.Ret.
+
+Definition bind {A B E : Type} (m : monad E A) (f : A -> monad E B) : monad E B := I.iMon_bind m f.
+#[warnings="-notation-overridden"]
+Notation "m >>= f" := (bind m f) (at level 50, left associativity).
+Definition bind0 {A E} (m : monad E unit) (n : monad E A) :=
+  m >>= fun (_ : unit) => n.
+#[warnings="-notation-overridden"]
+Notation "m >> n" := (bind0 m n) (at level 50, left associativity).
+
+Definition fail {A E} (msg : string) : monad E A :=
+  I.Next (I.GenericFail msg) (fun f => match f with end).
+
+Definition exit {A E} (_ : unit) : monad E A := fail "exit".
+
+Definition choose_bool {E} (_descr : string) : monad E bool := I.Next (I.Choose ChooseBool) mret.
+Definition choose_bit {E} (_descr : string) : monad E bitU := I.Next (I.Choose ChooseBit) mret.
+Definition choose_int {E} (_descr : string) : monad E Z := I.Next (I.Choose ChooseInt) mret.
+Definition choose_nat {E} (_descr : string) : monad E Z := I.Next (I.Choose ChooseNat) mret.
+Definition choose_real {E} (_descr : string) : monad E R := I.Next (I.Choose ChooseReal) mret.
+Definition choose_string {E} (_descr : string) : monad E string := I.Next (I.Choose ChooseString) mret.
+Definition choose_range {E} (_descr : string) (lo hi : Z) : monad E Z := I.Next (I.Choose (ChooseRange lo hi)) mret.
+Definition choose_bitvector {E} (_descr : string) (n : Z) : monad E (mword n) :=
+  I.Next (I.Choose (ChooseBitvector n)) mret.
+(* match n return monad (mword n) E with
+ | Zneg _ => returnm (bv_0 0)
+ | Z0 => returnm (bv_0 0)
+ | Zpos p => I.Next (I.Choose (N.of_nat (Pos.to_nat p))) (fun bv => returnm bv)
+ end.*)
+
+Definition assert_exp {E} (exp :bool) msg : monad E unit :=
+ if exp then returnm tt else fail msg.
+Definition assert_exp' {E} (exp :bool) msg : monad E (exp = true) :=
+ if exp return monad E (exp = true) then returnm eq_refl else fail msg.
+
+Definition throw {A E} (e : E) : monad E A := I.Next (I.ExtraOutcome e) mret.
+
+Fixpoint try_catch {A E1 E2} (m : monad E1 A) (h : E1 -> monad E2 A) : monad E2 A :=
+  match m with
+  | I.Ret r => I.Ret r
+  | I.Next (I.ExtraOutcome e)                  _ => h e
+  | I.Next (I.RegRead reg direct)              f => I.Next (I.RegRead reg direct) (fun t => try_catch (f t) h)
+  | I.Next (I.RegWrite reg direct regval)      f => I.Next (I.RegWrite reg direct regval) (fun t => try_catch (f t) h)
+  | I.Next (I.MemRead n nt req)                f => I.Next (I.MemRead n nt req) (fun t => try_catch (f t) h)
+  | I.Next (I.MemWrite n nt req)               f => I.Next (I.MemWrite n nt req) (fun t => try_catch (f t) h)
+  | I.Next (I.InstrAnnounce opcode)            f => I.Next (I.InstrAnnounce opcode) (fun t => try_catch (f t) h)
+  | I.Next (I.BranchAnnounce sz pa)            f => I.Next (I.BranchAnnounce sz pa) (fun t => try_catch (f t) h)
+  | I.Next (I.Barrier barrier)                 f => I.Next (I.Barrier barrier) (fun t => try_catch (f t) h)
+  | I.Next (I.CacheOp op)                      f => I.Next (I.CacheOp op) (fun t => try_catch (f t) h)
+  | I.Next (I.TlbOp op)                        f => I.Next (I.TlbOp op) (fun t => try_catch (f t) h)
+  | I.Next (I.TakeException fault)             f => I.Next (I.TakeException fault) (fun t => try_catch (f t) h)
+  | I.Next  I.ReturnException                  f => I.Next  I.ReturnException (fun t => try_catch (f t) h)
+  | I.Next (I.TranslationStart ts)             f => I.Next (I.TranslationStart ts) (fun t => try_catch (f t) h)
+  | I.Next (I.TranslationEnd te)               f => I.Next (I.TranslationEnd te) (fun t => try_catch (f t) h)
+  | I.Next (I.GenericFail msg)                 f => I.Next (I.GenericFail msg) (fun t => try_catch (f t) h)
+  | I.Next  I.CycleCount                       f => I.Next  I.CycleCount (fun t => try_catch (f t) h)
+  | I.Next  I.GetCycleCount                    f => I.Next  I.GetCycleCount (fun t => try_catch (f t) h)
+  | I.Next (I.Choose n)                        f => I.Next (I.Choose n) (fun t => try_catch (f t) h)
+  | I.Next (I.Discard)                         f => I.Next (I.Discard) (fun t => try_catch (f t) h)
+  | I.Next (I.Message msg)                     f => I.Next (I.Message msg) (fun t => try_catch (f t) h)
+  end.
+
+Definition early_return {A R E} (r : R) : monadR R E A := throw (inl r).
+Definition catch_early_return {A E} (m : monadR A E A) : monad E A :=
+  try_catch m
+    (fun r => match r with
+      | inl a => returnm a
+      | inr e => throw e
+     end).
+
+Definition pure_early_return_bind {A B E} (v : E + A) (f : A -> E + B) : E + B :=
+  match v with
+  | inl e => inl e
+  | inr a => f a
+  end.
+
+#[warnings="-notation-overridden"]
+Notation "m >>$= f" := (pure_early_return_bind m f) (at level 50, left associativity).
+#[warnings="-notation-overridden"]
+Notation "m >>$ n" := (m >>$= fun _ => n) (at level 50, left associativity).
+
+Definition pure_early_return {A} (v : A + A) : A :=
+  match v with
+  | inl v' => v'
+  | inr v' => v'
+  end.
+
+(* Lift to monad with early return by wrapping exceptions *)
+Definition liftR {A R E} (m : monad E A) : monadR R E A :=
+ try_catch m (fun e => throw (inr e)).
+
+Definition pure_early_return_embed {A R E} (v : R + A) : monadR R E A :=
+  match v with
+  | inl v' => early_return v'
+  | inr v' => returnm v'
+  end.
+
+(* Catch exceptions in the presence : early returns *)
+Definition try_catchR {A R E} (m : monadR R E A) (h : E -> monadR R E A) :=
+  try_catch m
+    (fun r => match r with
+      | inl r => throw (inl r)
+      | inr e => h e
+     end).
+
+
+
+Section Undef.
+
+Definition undefined_unit {E} (_:unit) : monad E unit := returnm tt.
+Definition undefined_bool {E} (_:unit) : monad E bool := choose_bool "undefined_bool".
+Definition undefined_bit {E} (_:unit) : monad E bitU := choose_bool "undefined_bit" >>= fun b => returnm (bitU_of_bool b).
+Definition undefined_string {E} (_:unit) : monad E string := choose_string "undefined_string".
+ Definition undefined_int {E} (_:unit) : monad E Z := choose_int "undefined_int".
+Definition undefined_nat {E} (_:unit) : monad E Z := choose_nat "undefined_nat".
+Definition undefined_real {E} (_:unit) : monad E _ := choose_real "undefined_real".
+Definition undefined_range {E} i j : monad E Z := choose_range "undefined_range" i j.
+Definition undefined_bitvector {E} n : monad E (mword n) := choose_bitvector "undefined_bitvector" n.
+
+Definition undefined_vector {E T} n `{Inhabited T} (a:T) : monad E (vec T n) := returnm (vector_init n a).
+
+End Undef.
+
+(* ---- Prompt_monad *)
+
+Definition read_reg {a e} (reg : A.reg a) : monad e a :=
+  let k v := I.Ret v in
+  I.Next (I.RegRead reg None) k.
+
+Definition read_reg_ref {a e} (ref : register_ref A.reg a) : monad e a :=
+  let k v := I.Ret v in
+  I.Next (I.RegRead ref.(Values.reg) None) k.
+
+Definition reg_deref {a e} := @read_reg_ref a e.
+
+Definition write_reg {a e} (reg : A.reg a) (v : a) : monad e unit :=
+ I.Next (I.RegWrite reg None v) I.Ret.
+
+Definition write_reg_ref {a e} (ref : register_ref A.reg a) (v : a) : monad e unit :=
+ I.Next (I.RegWrite ref.(Values.reg) None v) I.Ret.
+
+(* ---- Prompt *)
+
+Fixpoint foreachM {a e Vars} (l : list a) (vars : Vars) (body : a -> Vars -> monad e Vars) : monad e Vars :=
+match l with
+| [] => returnm vars
+| (x :: xs) =>
+  body x vars >>= fun vars =>
+  foreachM xs vars body
+end.
+
+Fixpoint foreachE {a Vars e} (l : list a) (vars : Vars) (body : a -> Vars -> e + Vars) : e + Vars :=
+match l with
+| [] => inr vars
+| (x :: xs) =>
+  body x vars >>$= fun vars =>
+  foreachE xs vars body
+end.
+
+Fixpoint foreach_ZM_up' {E Vars} (from to step off : Z) (n : nat) (* 0 <? step *) (* 0 <=? off *) (vars : Vars) (body : forall (z : Z) (* from <=? z <=? to *), Vars -> monad E Vars) {struct n} : monad E Vars :=
+  if sumbool_of_bool (from + off <=? to) then
+    match n with
+    | O => returnm vars
+    | S n => body (from + off) vars >>= fun vars => foreach_ZM_up' from to step (off + step) n vars body
+    end
+  else returnm vars.
+
+Fixpoint foreach_ZE_up' {e Vars} (from to step off : Z) (n : nat) (* 0 <? step *) (* 0 <=? off *) (vars : Vars) (body : forall (z : Z) (* from <=? z <=? to *), Vars -> e + Vars) {struct n} : e + Vars :=
+  if sumbool_of_bool (from + off <=? to) then
+    match n with
+    | O => inr vars
+    | S n => body (from + off) vars >>$= fun vars => foreach_ZE_up' from to step (off + step) n vars body
+    end
+  else inr vars.
+
+Fixpoint foreach_ZM_down' {E Vars} (from to step off : Z) (n : nat) (* 0 <? step *) (* off <=? 0 *) (vars : Vars) (body : forall (z : Z) (* to <=? z <=? from *), Vars -> monad E Vars) {struct n} : monad E Vars :=
+  if sumbool_of_bool (to <=? from + off) then
+    match n with
+    | O => returnm vars
+    | S n => body (from + off) vars >>= fun vars => foreach_ZM_down' from to step (off - step) n vars body
+    end
+  else returnm vars.
+
+Fixpoint foreach_ZE_down' {e Vars} (from to step off : Z) (n : nat) (* 0 <? step *) (* off <=? 0 *) (vars : Vars) (body : forall (z : Z) (* to <=? z <=? from *), Vars -> e + Vars) {struct n} : e + Vars :=
+  if sumbool_of_bool (to <=? from + off) then
+    match n with
+    | O => inr vars
+    | S n => body (from + off) vars >>$= fun vars => foreach_ZE_down' from to step (off - step) n vars body
+    end
+  else inr vars.
+
+Definition foreach_ZM_up {E Vars} from to step vars body (* 0 <? step *) :=
+    foreach_ZM_up' (E := E) (Vars := Vars) from to step 0 (S (Z.abs_nat (from - to))) vars body.
+Definition foreach_ZM_down {E Vars} from to step vars body (* 0 <? step *) :=
+    foreach_ZM_down' (E := E) (Vars := Vars) from to step 0 (S (Z.abs_nat (from - to))) vars body.
+
+Definition foreach_ZE_up {e Vars} from to step vars body (* 0 <? step *) :=
+    foreach_ZE_up' (e := e) (Vars := Vars) from to step 0 (S (Z.abs_nat (from - to))) vars body.
+Definition foreach_ZE_down {e Vars} from to step vars body (* 0 <? step *) :=
+    foreach_ZE_down' (e := e) (Vars := Vars) from to step 0 (S (Z.abs_nat (from - to))) vars body.
+
+Definition genlistM {A E} (f : nat -> monad E A) (n : nat) : monad E (list A) :=
+  let indices := List.seq 0 n in
+  foreachM indices [] (fun n xs => (f n >>= (fun x => returnm (xs ++ [x])%list))).
+
+Definition and_boolM {E} (l : monad E bool) (r : monad E bool) : monad E bool :=
+ l >>= (fun l => if l then r else returnm false).
+
+Definition or_boolM {E} (l : monad E bool) (r : monad E bool) : monad E bool :=
+ l >>= (fun l => if l then returnm true else r).
+
+
+(* For termination of recursive functions. *)
+Definition _limit_reduces {_limit} (_acc:Acc (Zwf 0) _limit) (H : _limit >= 0) : Acc (Zwf 0) (_limit - 1).
+refine (Acc_inv _acc _).
+unbool_comparisons.
+red.
+Lia.lia.
+Defined.
+
+(* A version of well-foundedness of measures with a guard to ensure that
+   definitions can be reduced without inspecting proofs, based on a coq-club
+   thread featuring Barras, Gonthier and Gregoire, see
+     https://sympa.inria.fr/sympa/arc/coq-club/2007-07/msg00014.html *)
+
+Fixpoint pos_guard_wf {A:Type} {R:A -> A -> Prop} (p:positive) : well_founded R -> well_founded R :=
+ match p with
+ | xH => fun wfR x => Acc_intro x (fun y _ => wfR y)
+ | xO p' => fun wfR x => let F := pos_guard_wf p' in Acc_intro x (fun y _ => F (F 
+wfR) y)
+ | xI p' => fun wfR x => let F := pos_guard_wf p' in Acc_intro x (fun y _ => F (F 
+wfR) y)
+ end.
+
+Definition Zwf_guarded (z:Z) : Acc (Zwf 0) z :=
+  Acc_intro _ (fun y H => match z with
+  | Zpos p => pos_guard_wf p (Zwf_well_founded _) _
+  | Zneg p => pos_guard_wf p (Zwf_well_founded _) _
+  | Z0 => Zwf_well_founded _ _
+  end).
+
+(*val whileM : forall 'rv 'vars 'e. 'vars -> ('vars -> monad 'rv bool 'e) ->
+                ('vars -> monad 'rv 'vars 'e) -> monad 'rv 'vars 'e*)
+Fixpoint whileMT' {E Vars} limit (vars : Vars) (cond : Vars -> monad E bool) (body : Vars -> monad E Vars) (acc : Acc (Zwf 0) limit) : monad E Vars.
+exact (
+  if Z_ge_dec limit 0 then
+    cond vars >>= fun cond_val =>
+    if cond_val then
+      body vars >>= fun vars => whileMT' _ _ (limit - 1) vars cond body (_limit_reduces acc ltac:(assumption))
+    else returnm vars
+  else fail "Termination limit reached").
+Defined.
+
+Definition whileMT {E Vars} (vars : Vars) (measure : Vars -> Z) (cond : Vars -> monad E bool) (body : Vars -> monad E Vars) : monad E Vars :=
+  let limit := measure vars in
+  whileMT' limit vars cond body (Zwf_guarded limit).
+
+Fixpoint untilMT' {E Vars} limit (vars : Vars) (cond : Vars -> monad E bool) (body : Vars -> monad E Vars) (acc : Acc (Zwf 0) limit) : monad E Vars.
+exact (
+  if Z_ge_dec limit 0 then
+    body vars >>= fun vars =>
+    cond vars >>= fun cond_val =>
+    if cond_val then returnm vars else untilMT' _ _ (limit - 1) vars cond body (_limit_reduces acc ltac:(assumption))
+  else fail "Termination limit reached").
+Defined.
+
+Definition untilMT {E Vars} (vars : Vars) (measure : Vars -> Z) (cond : Vars -> monad E bool) (body : Vars -> monad E Vars) : monad E Vars :=
+  let limit := measure vars in
+  untilMT' limit vars cond body (Zwf_guarded limit).
+
+Section Choose.
+
+Definition choose_from_list {A E} (descr : string) (xs : list A) : monad E A :=
+  (* Use sufficiently many nondeterministically chosen bits and convert into an
+     index into the list *)
+  choose_range descr 0 (Z.of_nat (List.length xs) - 1) >>= fun idx =>
+  match List.nth_error xs (Z.to_nat idx) with
+    | Some x => returnm x
+    | None => fail ("choose " ++ descr)
+  end.
+
+Definition internal_pick {a e} (xs : list a) : monad e a :=
+  choose_from_list "internal_pick" xs.
+
+End Choose.
+
+(* --- Operators_mwords.v *)
+
+Definition autocast_m {e m n} {T : Z -> Type} `{H : Inhabited (T n)} (x : monad e (T m)) : monad e (T n) :=
+  x >>= fun x => returnm (autocast x).
+
+(* --- should probably define generic versions of these, parametrised by Arch *)
+
+Definition sail_barrier {e} (b : A.barrier) : monad e unit :=
+  I.Next (I.Barrier b) I.Ret.
+
+Definition sail_take_exception {e} (f : A.fault) : monad e unit :=
+  I.Next (I.TakeException f) I.Ret.
+
+Definition sail_return_exception {e} (_:unit) : monad e unit :=
+  I.Next I.ReturnException I.Ret.
+
+Definition sail_cache_op {e} (op : A.cache_op) : monad e unit :=
+  I.Next (I.CacheOp op) I.Ret.
+
+Definition sail_tlbi {e} (op : A.tlb_op) : monad e unit :=
+  I.Next (I.TlbOp op) I.Ret.
+
+Definition branch_announce {e} sz (addr : mword sz) : monad e unit :=
+  (* TODO: branch_announce seems rather odd *)
+  I.Next (I.BranchAnnounce sz addr) I.Ret.
+
+Definition instr_announce {e sz} (opcode : mword sz) : monad e unit :=
+  I.Next (I.InstrAnnounce (bv_to_bvn (get_word opcode))) I.Ret.
+
+Definition cycle_count {e} (_ : unit) : monad e unit := I.Next I.CycleCount I.Ret.
+Definition get_cycle_count {e} (_ : unit) : monad e Z := I.Next I.GetCycleCount I.Ret.
+
+(* TODO: check endianness *)
+Definition bytes_of_bv {n} (v : bv (8 * Z.to_N n)) : vec (bv 8) n :=
+  vec_init_fn n (fun i => bv_extract (8 * Z.to_N i) 8 v).
+
+Definition bools_of_bv {n} (v : bv (Z.to_N n)) : vec bool n :=
+  vec_init_fn n (fun i => MachineWord.MachineWord.get_bit v (Z.to_N i)).
+
+Definition sail_mem_read {e n nt} (req : Mem_read_request n nt (Z.of_N A.addr_size) A.addr_space A.mem_acc) : monad e (result (vec (mword 8) n * vec bool nt) A.abort) :=
+  let n' := Z.to_N n in
+  let nt' := Z.to_N nt in
+  let address := cast_N req.(Mem_read_request_address) (N2Z.id _) in
+  let req' := I.ReadReq.make n' nt' req.(Mem_read_request_access_kind) address req.(Mem_read_request_address_space) in
+  let k r :=
+    match r with
+    | inl (x,y) =>
+        I.Ret (Ok (bytes_of_bv x, bools_of_bv y))
+    | inr abort => I.Ret (Err abort)
+    end
+  in
+  I.Next (I.MemRead n' nt' req') k.
+
+Definition bv_of_bytes {n} (v : vec (bv 8) n) : bv (8 * Z.to_N n).
+refine (
+  cast_N (list_rec (fun l => bv (8 * N.of_nat (length l))) (bv_0 0) (fun v _ t => bv_concat _ v t) (projT1 v)) _
+).
+destruct v as [l H].
+simpl.
+rewrite H.
+rewrite Z_nat_N.
+reflexivity.
+Defined.
+
+Definition bv_of_bools {n} (v : vec bool n) : bv (Z.to_N n) := of_bools (projT1 v).
+
+Definition sail_mem_write {e n nt} (req : Mem_write_request n nt (Z.of_N A.addr_size) A.addr_space A.mem_acc) : monad e (result unit A.abort) :=
+  let n' := Z.to_N n in
+  let nt' := Z.to_N nt in
+  let value := bv_of_bytes req.(Mem_write_request_value) in
+  let address := cast_N req.(Mem_write_request_address) (N2Z.id _) in
+  let address_space := req.(Mem_write_request_address_space) in
+  let tags := bv_of_bools req.(Mem_write_request_tags) in
+  let access_kind := req.(Mem_write_request_access_kind) in
+  let req' := I.WriteReq.make n' nt' access_kind address address_space value tags in
+  let k x :=
+    match x with
+    | inl _ => I.Ret (Ok tt)
+    | inr y => I.Ret (Err y)
+    end
+  in
+  I.Next (I.MemWrite n' nt' req') k.
+
+Definition sail_sys_reg_read {e T} (id : A.sys_reg_id) (r : register_ref A.reg T) : monad e T :=
+  I.Next (I.RegRead r.(Values.reg) (Some id)) I.Ret.
+
+Definition sail_sys_reg_write {e T} (id : A.sys_reg_id) (r : register_ref A.reg T) (v : T) : monad e unit :=
+  I.Next (I.RegWrite r.(Values.reg) (Some id) v) I.Ret.
+
+Definition sail_translation_start {e} (ts : A.trans_start) : monad e unit := I.Next (I.TranslationStart ts) I.Ret.
+Definition sail_translation_end {e} (te : A.trans_end) : monad e unit := I.Next (I.TranslationEnd te) I.Ret.
+
+(* ----------- *)
+(* The normal print routines do nothing in Coq so that they don't drag terms and functions into the
+   monad.  Here are alternative versions which do, which can be controlled by defining PRINT_EFFECTS
+   in Sail. *)
+Definition print_effect {e} (s : string) : monad e unit :=
+  I.Next (I.Message s) I.Ret.
+
+Definition print_endline_effect {e} (s : string) : monad e unit :=
+  print_effect (s ++ "
+")%string.
+
+Definition print_int_effect {e} s i : monad e unit :=
+  print_endline_effect (s ++ string_of_int i).
+
+Definition print_bits_effect {e n} s (w : mword n) : monad e unit :=
+  print_endline_effect (s ++ string_of_bits w).
+
+(* We only have one output stream that we use for both. *)
+Definition prerr_effect {e} s := @print_effect e s.
+Definition prerr_endline_effect {e} s := @print_endline_effect e s.
+Definition prerr_int_effect {e} s i := @print_int_effect e s i.
+Definition prerr_bits_effect {e} s i := @print_bits_effect e s i.
+
+End Defs.
